<?xml version='1.0' encoding='utf-8'?>
<section xml:id="sec_5-2_5-3_exponential-limits-derivatives" xmlns:xi="http://www.w3.org/2001/XInclude">

  <title>Section 5.2 &amp; 5.3: Exponential and Logarithmic Limits and Derivatives</title>

  <slide>
    <title>Learning Goals</title>

    <ul>
      <li>
        <p>
          Compute end behavior for exponential and logarithmic functions, using the ideas of exponential growth vs decay and the inverse property for logarithms.
        </p>
      </li>
      <li>
        <p>
          Recognize how the derivatives of the exponential and logarithm come from the definition of the derivative and the properties of derivatives.
        </p>
      </li>
      <li>
        <p>
          Compute derivatives using derivative rules involving the natural exponential and logarithm function, including the use of other derivative rules (product, quotient, chain).
        </p>
      </li>
      <li>
        <p>
          Shapes of graphs based on derivative sign analysis.
        </p>
      </li>
    </ul>
  </slide>

  <slide>
    <title>Exponential Functions and Limits</title>

    <ul>
      <li>
        <p>
          <em>Core Fact</em>: Exponential functions are <term>continuous</term>, so we evaluate limits at points with simple evaluation.
          As the inverse of a monotonic continuous function, the logarithm must also be continuous.
        </p>
      </li>
      <li>
        <p>
          Think about the graph of exponential growth and decay to determine limits as <m>x \to \pm \infty</m>.
          <ul>
            <li>
              <p>
                If <m>b &gt; 1</m>, then <m>b^x</m> is exponential growth and limits <m>b^{-\infty} = 0</m> and <m>b^{\infty} = \infty</m>.
              </p>
              <image width="30%">
                <shortdescription>Graph of exponential growth with b &gt; 1 so that y tends to 0 on the left and to infinity on the right.</shortdescription>
                <latex-image>
                  \begin{tikzpicture}
                    \begin{axis}[
                        axis lines = middle,
                        grid = both,
                        xmin = -3,
                        xmax = 3,
                        ymin = -1,
                        ymax = 10,
                        width=8cm,
                        height=8cm,
                        xlabel={$x$},
                        ylabel={$y$}
                      ]
                      \addplot[
                        domain=-3:3,
                        blue,
                        samples=200, 
                        line width=2pt
                      ]
                      {2^x};
                    \end{axis}
                  \end{tikzpicture}
                </latex-image>
              </image>
            </li>
            <li>
              <p>
                If <m>0 &lt; b &lt; 1</m>, then <m>b^x</m> is exponential decay and limits <m>b^{-\infty} = \infty</m> and <m>b^{\infty} = 0</m>.
              </p>
            </li>
          </ul>
        </p>
      <image width="30%">
        <shortdescription>Graph of exponential growth with 0 &lt; b &lt; 1 so that y tends to infinity on the left and to 0 on the right.</shortdescription>
        <latex-image>
          \begin{tikzpicture}
            \begin{axis}[
                axis lines = middle,
                grid = both,
                xmin = -3,
                xmax = 3,
                ymin = -1,
                ymax = 10,
                width=8cm,
                height=8cm, 
                xlabel={$x$},
                ylabel={$y$}
              ]
              \addplot[
                domain=-3:3,
                blue,
                samples=200, 
                line width=2pt
              ]
              {2^(-x)};
            \end{axis}
          \end{tikzpicture}
        </latex-image>
      </image>
      </li>
    </ul>
  </slide>

  <slide>
    <title>Derivative of Exponential</title>
    
    <p>
      For each new function, we need to use the definition of the derivative to discover the corresponding derivative rule.
      <md>
        f'(x) = \lim_{h \to 0}\frac{f(x+h)-f(x)}{h}
      </md>
      When <m>f(x) = b^x</m>, we use the exponent sum rule to rewrite <m>f(x+h) = b^{x+h} = b^x \cdot b^h</m>:
      <md>
        <mrow>f'(x) &amp;= \lim_{h \to 0} \frac{b^{x+h}-b^x}{h} = \lim_{h \to 0} \frac{b^x b^h - b^x}{h}</mrow>
        <mrow> &amp;= \lim_{h \to 0} \frac{b^x(b^h-1)}{h} = b^x \cdot \lim_{h \to 0} \frac{b^h - 1}{h}</mrow>
      </md>
      Consequently, the derivative of an elementary exponential is always some constant <m>L(b)</m> times the original function <m>b^x</m>, where
      <md>L(b) = \lim_{h \to 0}\frac{b^h-1}{h}</md>
    </p>
  </slide>
  <slide>
    <title>Natural Base <m>e</m></title>
    
    <p>
      The value of <m>L(b)</m> is exactly the value of the derivative of <m>b^x</m> at <m>x=0</m>.
      Different bases have different slopes at this point.
    </p>
    <p>
      The base <m>e</m> is that number such that <m>L(b) = 1</m> so that the tangent line is exactly <m>y=1+x</m>:
      <md>
        \lim_{h \to 0} \frac{e^h - 1}{h} = \lim_{x \to 0} \frac{e^x - 1}{x} = 1.
      </md>
      The value as a decimal approximation is <m>e \approx 2.71828183</m>.
    </p>

    <p>
      Since <m>L(e) = 1</m>, we have the remarkable derivative rule <m>\frac{d}{dx}[e^x] = e^x</m>.
      Incorporating the chain rule, for any formula <m>u</m>, we have
      <md>\frac{d}{dx}[e^u] = e^u \cdot u'</md>.
    </p>
  </slide>

  <slide>
    <title>Practice Derivatives</title>
    
    <p>
      Find the derivatives of the following functions.
      <ol>
        <li><p><m>f(x) = x^2 e^{x}</m></p></li>
        <li><p><m>g(x) = 3e^{-2x}</m></p></li>
        <li><p><m>h(x) = x e^{-x^2}</m></p></li>
      </ol>
    </p>    
  </slide>


  <slide>
    <title>The Natural Logarithm</title>
    
    <p>
      Now that we have defined the natural base <m>e</m>, we can also define the <term>natural logarithm</term>,
      which is the inverse function to <m>y=e^x</m>:
      <md>\ln(e^x) = x \qquad \text{and} \qquad e^{\ln(x)} = x</md>.
    </p>

    <p>
      Like <em>all logarithms</em>, we have <m>\ln(1) = 0</m>.
    </p>
    <p>
      Because <m>e &gt;1</m>, we also have <m>\ln(x) &lt; 0 </m> for <m>0 &lt; x &lt; 1</m>
      and <m>\ln(x) &gt; 0</m> for <m>x &gt; 1</m>.
    </p>
  </slide>

  <slide>
    <title>The Natural Logarithm's Derivative</title>
    <p>
      To find <m>\ln'(x)</m>, we will do the same approach as for <em>all</em> inverse functions<mdash/>use implicit differentiation:
      <md>
        <mrow>y = \ln(x) \quad \Leftrightarrow \quad e^y = x</mrow>
        <mrow>\frac{d}{dx}[e^y] = \frac{d}{dx}[x]</mrow>
        <mrow>e^y \cdot y' = 1</mrow>
        <mrow>y' = \frac{1}{e^y} = \frac{1}{x}</mrow>
      </md>
      That is, <m>\ln'(x) = \frac{1}{x}</m>, and for <em>any</em> expression <m>u</m>, the chain rule gives:
      <md>
        \frac{d}{dx}\ln(u) = \ln'(u) \cdot u' = \frac{1}{u} \cdot u' = \frac{u'}{u}
      </md>
      
    </p>
  </slide>

</section>
